<?xml version="1.0"?>

<!DOCTYPE rdf:RDF [
 <!ENTITY rdf 'http://www.w3.org/1999/02/22-rdf-syntax-ns#'>
 <!ENTITY rdfs 'http://www.w3.org/2000/01/rdf-schema#'>
 <!ENTITY mulgara 'http://mulgara.org/mulgara#'>
]>

<rdf:RDF xml:base="http://mulgara.org/mulgara" xml:lang="en"
  xmlns:rdf="&rdf;"
  xmlns:rdfs="&rdfs;"
  xmlns:mulgara="&mulgara;" >

<rdfs:Class rdf:ID="Model"
  rdfs:label="Model"
  rdfs:comment="A set of rdf:Statements">
</rdfs:Class>

<!-- A reified RDF Statement is a mulgara Model with a single statement -->
<rdfs:Class rdf:about="&rdf;Statement">
  <rdfs:subClassOf rdf:resource="&mulgara;Model"/>
</rdfs:Class>

<rdfs:Class rdf:ID="LuceneModel"
  rdfs:label="Lucene model"
  rdfs:comment="A model backed by a Lucene full text index">
  <rdfs:subclassOf rdf:resource="#Model"/>
</rdfs:Class>


<!--========== LDAP Authentication / mulgara Authorization ============-->
<!-- 
Use Principals to define Permissions when using LDAP for authentication. 

Principals are assigned URLs. The scheme part is "java:" and the path 
part is the classname of an implementation of java.security.Principal, 
followed by a "/" and trailing data which is parsed into arguments for the 
class constructor.

Example: java:com.sun.security.auth.UnixPrincipal/jsmith

An example config is in data/security-unix.rdf. If using mulgara for 
authentication see the section below.
-->

<rdfs:Class rdf:ID="Principal"
  rdfs:label="Principal"
  rdfs:comment="A credential such as a unique name or group membership">
</rdfs:Class>



<!--===========  mulgara Authentication/ mulgara Authorization  ===========-->

<!--
Use 'Group' and 'User' definitions to specify Permissions when using mulgara for 
authentication and authorization.

Groups and Users are assigned URLs. The scheme part is "mulgara:" and the path 
part is ether 'group' or 'user', followed by a "/" and then the name of the 
group or the username of the user.

Example: mulgara:group/dev or mulgara:user/fred

An example config file is in data/security-mulgara.rdf. If using LDAP for 
authentication see the section above.
-->

<!-- User Group - subclass of Principal -->

<rdfs:Class rdf:ID="Group"
  rdfs:label="Group"
  rdfs:comment="A user group for providing a common set of permissions to a group of users">
  <rdfs:subclassOf rdf:resource="#Principal"/>
</rdfs:Class>

<rdf:Property rdf:ID="groupname"
  rdfs:label="Name"
  rdfs:comment="The group's name">
  <rdfs:domain rdf:resource="#Group"/>
  <rdfs:range rdf:resource="&rdfs;Literal"/>
</rdf:Property>


<!-- User - subclass of Principal -->

<rdfs:Class rdf:ID="User"
  rdfs:label="User"
  rdfs:comment="A mulgara user">
  <rdfs:subclassOf rdf:resource="#Principal"/>
</rdfs:Class>

<rdf:Property rdf:ID="username"
  rdfs:label="Username"
  rdfs:comment="A user's username">
  <rdfs:domain rdf:resource="#User"/>
  <rdfs:range rdf:resource="&rdfs;Literal"/>
</rdf:Property>

<rdf:Property rdf:ID="password" 
  rdfs:label="Password"
  rdfs:comment="A user's password">
  <rdfs:domain rdf:resource="#User"/>
  <rdfs:range rdf:resource="&rdfs;Literal"/>
</rdf:Property>

<rdf:Property rdf:ID="group" 
  rdfs:label="User Group"
  rdfs:comment="A user group that the user belongs to">
  <rdfs:domain rdf:resource="#User"/>
  <rdfs:range rdf:resource="#Group"/>
</rdf:Property>



<!--======================  Permissions  ======================-->

<!-- All instances of mulgara:Permission should have a domain of mulgara:Principal and
     a range of mulgara:Model. -->
<rdfs:Class rdf:ID="Permission" 
  rdfs:label="Permission"
  rdfs:comment="The four RDF properties mulgara:canRead, mulgara:canWrite, mulgara:canCreate and mulgara:canDelete">
  <rdfs:subclassOf rdf:resource="&rdf;Property"/>
</rdfs:Class>

<mulgara:Permission rdf:ID="canCreate"
  rdfs:label="can create"
  rdfs:comment="Permission for a mulgara:Principal (the subject) to create a mulgara:Model from a specified rdf:Resource (the object)">
  <rdfs:domain rdf:resource="&mulgara;Principal"/>
  <rdfs:range rdf:resource="&mulgara;Model"/>
</mulgara:Permission>

<mulgara:Permission rdf:ID="canDelete"
  rdfs:label="can delete"
  rdfs:comment="Permission for a mulgara:Principal (the subject) to remove a mulgara:Model (the object)">
  <rdfs:domain rdf:resource="&mulgara;Principal"/>
  <rdfs:range rdf:resource="&mulgara;Model"/>
</mulgara:Permission>

<mulgara:Permission rdf:ID="canRead"
  rdfs:label="can read"
  rdfs:comment="Permission for a mulgara:Principal (the subject) to know if a statement occurs within a mulgara:Model (the object)">
  <rdfs:domain rdf:resource="&mulgara;Principal"/>
  <rdfs:range rdf:resource="&mulgara;Model"/>
</mulgara:Permission>

<mulgara:Permission rdf:ID="canWrite"
  rdfs:label="can write"
  rdfs:comment="Permission for a mulgara:Principal (the subject) to modify the occurence of statements within a mulgara:Model (the object)">
  <rdfs:domain rdf:resource="&mulgara;Principal"/>
  <rdfs:range rdf:resource="&mulgara;Model"/>
</mulgara:Permission>

</rdf:RDF>

